

Answer Key and Marking Scheme

Q1 Alternative approaches would also be accepted and awarded marks

- a The data scientist has the following plan in mind: the $D \times N$ data matrix X is modified to RX where R is a diagonal matrix with $R_{ii} = \alpha_i$ to get the modified data matrix. The original covariance matrix XX^T could be written as $S\Lambda S^T$ using the spectral theorem. Now the covariance matrix for the modified data matrix RX can be written as RXX^TR^T which can be written as $RS\Lambda S^TR^T$. This might give the impression that the spectral decomposition of RXX^TR^T is $RS\Lambda S^TR^T$ where RS plays the role of the eigenvector matrix. However, we see that RS is not an orthogonal matrix since $RSS^TR^T = RR^T \neq I$. If RS had been an orthogonal matrix, the data scientist's claims would have been true, but this is not the case.

Marking Scheme: 3 Marks \rightarrow factoring the modified covariance matrix, 2 Marks \rightarrow the rest of the argument.

- b The $D \times N$ data matrix X after transformation becomes RX where R is a diagonal matrix with $R_{ii} = \alpha_i$. The covariance matrix for this modified matrix becomes RXX^TR^T . Now XX^T is the previously computed covariance matrix, and we need to post-multiply it with a diagonal matrix R^T . The first column of the product XX^TR^T can be computed by taking a linear combination of the columns of XX^T with the combining coefficients coming from the first column of R^T . But the first column of R^T has a non-zero in only one place, ie the first location, so this linear combination can be computed in $O(D)$ time. Similarly the other columns of XX^TR^T can each be computed in $O(D)$ time, so that computing the whole matrix XX^TR^T takes $O(D^2)$ time. Computing RXX^TR^T means pre-multiplying the matrix XX^TR^T by the diagonal matrix R . The first row of RXX^TR^T can be obtained by taking a linear combination of the rows of XX^TR^T where the combining coefficients come from the first row of R . Since the first row of R has only a single non-zero entry, this boils down to a $O(D)$ computation. The other rows of XX^TR^T can be similarly computed, so the computation of RXX^TR^T can be seen to be of complexity $O(D^2) + O(D^2) = O(D^2)$.

Marking Scheme: 2 Marks \rightarrow recognizing the data matrix can be written as RX and XX^TR^T takes $O(D^2)$ time, 1 Mark \rightarrow the rest of the argument. If the student has pursued a different argument, partial marks to be awarded as necessary.

- c The Lagrangian expressed in terms of only the parameters α_i is the following $\alpha_1 + \alpha_2 + \alpha_3 - \frac{1}{2}(\sum_i \sum_j \alpha_i \alpha_j y_i y_j \mathbf{x}_i \cdot \mathbf{x}_j)$. In this case we see that this becomes $L = \alpha_1 + \alpha_2 + \alpha_3 - \frac{1}{2}(2\alpha_1\alpha_2(-1)(8) + 2\alpha_1\alpha_3(-1)(4) + 2\alpha_2\alpha_3(1)(2) + 10\alpha_1^2 + 10\alpha_2^2 + 2\alpha_3^2)$. We need to maximize this subject to the criterion that $\alpha_1 y_1 + \alpha_2 y_2 + \alpha_3 y_3 = 0$. This allows us to substitute for α_1 in terms of the other two variables α_2 and α_3 to get an expression in two variables. We simplify the expression L to $2(\alpha_2 + \alpha_3) + 8(\alpha_2 +$

$\alpha_3)\alpha_2 + 4(\alpha_2 + \alpha_3)\alpha_3 - 2\alpha_2\alpha_3 - 5(\alpha_2 + \alpha_3)^2 - 5\alpha_2^2 - 1\alpha_3^2$. This expression finally simplifies to $L = -2\alpha_2^2 - 2\alpha_3^2 + 2\alpha_2 + 2\alpha_3$. This has four terms in it and two variables. If you substitute for α_2 or α_3 in terms of the other variables, you still end up with four terms and two variables.

Using Calculus we can set $\frac{\partial L}{\partial \alpha_2} = 0$ to get $2 - 4\alpha_2 = 0$ or $\alpha_2 = 0.5$. Similarly $\frac{\partial L}{\partial \alpha_3} = 0$ gives $2 - 4\alpha_3 = 0$ which gives $\alpha_3 = 0.5$. From $\alpha_1 = \alpha_2 + \alpha_3$ we conclude $\alpha_1 = 1$. Now the vector $w = \alpha_1 y_1 \mathbf{x}_1 + \alpha_2 y_2 \mathbf{x}_2 + \alpha_3 y_3 \mathbf{x}_3 = 1 * 1[-1, 3]^T + 0.5 * -1 * [1, 3]^T + 0.5 * -1 * [-1, 1]^T = [-1, 1]$. Solving for b from $\mathbf{w}^T \mathbf{x} + b = 1$ at $\mathbf{x} = [-1, 3]^T$ gives $b = -3$. Thus the separating hyperplane is $-x_1 + x_2 - 3 = 0$.

Marking Scheme: 3 Marks \rightarrow obtaining the expression for the Lagrangian in terms of the α_i s. 2 Marks \rightarrow substituting for one of the α_i s in terms of the others and obtaining the simplest expression. 3 Marks \rightarrow taking partial derivatives, setting them to zero and computing the parameters.

Q2 Alternative approaches would also be accepted and awarded marks

2.1 (a)

$$\|\lambda x + (1 - \lambda)y\|_1 \leq \|\lambda x\|_1 + \|(1 - \lambda)y\|_1$$

In this step we used triangle inequality of ℓ_1 norm (1 marks).

Now rhs can be seen to satisfy the following

$$\|\lambda x\|_1 + \|(1 - \lambda)y\|_1 \leq |\lambda|\|x\|_1 + |(1 - \lambda)|\|y\|_1$$

In this step we used homogeneity of norms. (0.5 marks)

Hence, it can be seen that

$$\|\lambda x + (1 - \lambda)y\|_1 \leq \lambda\|x\|_1 + (1 - \lambda)\|y\|_1$$

This is the definition of convexity. Hence ℓ_1 norm is a convex function . (0.5 marks)

(b) We need to show that $h(x)$ satisfy the definition of convex function as discussed in course.

It can be seen by definition of $h(x)$ that

$$h(\lambda x + (1 - \lambda)y) = g\left(A(\lambda x + (1 - \lambda)y) + b\right) \quad (0.25marks)$$

we can simplify the expression as

$$g\left(A(\lambda x + (1 - \lambda)y) + b\right) = g\left(\lambda(Ax + b) + (1 - \lambda)(Ay + b)\right) \quad (0.5marks)$$

Since $g(x)$ is a convex function it satisfies the inequality

$$g\left(\lambda(Ax + b) + (1 - \lambda)(Ay + b)\right) \leq \lambda.g(Ax + b) + (1 - \lambda).g(Ay + b) \quad (0.5marks)$$

From definition of $h(x)$ we know that

$$\lambda.g(Ax + b) + (1 - \lambda).g(Ay + b) = \lambda.h(x) + (1 - \lambda).h(y) \quad (0.5marks)$$

Together from the previous 4 expressions, we can conclude that

$$h(\lambda x + (1 - \lambda)y) \leq \lambda h(x) + (1 - \lambda)h(y) \quad (0.25marks)$$

Hence $h(x)$ is a convex function . (2 marks)

2.2 Let the singular values of A in diagonal entries of Σ be named $\sigma_1, \sigma_2, \dots, \sigma_n$.

(a) By definition of Frobenius norm we get

$$\gamma = \sigma_1^2 + \sigma_2^2 + \dots + \sigma_n^2 \quad (0.5 \text{ marks})$$

Now, we can see the following

$$\alpha = \text{Tr}(B) = \text{Tr}(A^T A) = \text{Tr}(V \Sigma^T \Sigma V^T) = \text{Tr}(\Sigma^T \Sigma) = \sigma_1^2 + \sigma_2^2 + \dots + \sigma_n^2 = \gamma \quad (0.5 \text{ marks})$$

We have used property that $\text{Tr}(M_1 M_2) = \text{Tr}(M_2 M_1)$.

In conclusion claim made by G1 is True

(b) By definition of Frobenius norm we get

$$\gamma = \sigma_1^2 + \sigma_2^2 + \dots + \sigma_n^2 \quad (0.5 \text{ marks})$$

Now, we can see the following

$$\alpha = \text{Tr}(B) = \text{Tr}(A^T A) = \text{Tr}(V \Sigma^T \Sigma V^T) = \text{Tr}(\Sigma^T \Sigma) = \sigma_1^2 + \sigma_2^2 + \dots + \sigma_n^2 = \gamma \quad (0.5 \text{ marks})$$

We have used property that $\text{Tr}(M_1 M_2) = \text{Tr}(M_2 M_1)$.

In conclusion claim made by G2 is False

(c) By definition of Frobenius norm we get

$$\gamma = \sigma_1^2 + \sigma_2^2 + \dots + \sigma_n^2 \quad (0.5 \text{ marks})$$

Now, we can see the following

$$\beta = \text{Tr}(C) = \text{Tr}(A A^T) = \text{Tr}(U \Sigma^T \Sigma U^T) = \text{Tr}(\Sigma^T \Sigma) = \sigma_1^2 + \sigma_2^2 + \dots + \sigma_n^2 = \gamma \quad (1 \text{ mark})$$

We have used property that $\text{Tr}(M_1 M_2) = \text{Tr}(M_2 M_1)$.

In conclusion $\beta \neq \gamma^2$ (0.5 marks)

2.3 (a) First observe that

$$\|Ax - b\|_2^2 = x^T A^T A x - 2x^T A^T b + b^T b \quad (1 \text{ mark})$$

The gradient of the above part alone is easily derived based on identities learned in course as

$$2A^T A x - 2A^T b \quad (0.5 \text{ marks})$$

Now the gradient of the remaining part ie $c^T x + d$ is obtained as c (0.5 marks)

Hence $\nabla f(x) = 2A^T A x - 2A^T b + c$

(b) First observe that

$$\|A_1^T A_1 x\|_2^2 = x^T A_1^T A_1 A_1^T A_1 x \quad (0.5 \text{ marks})$$

The gradient of the above part alone is easily derived based on identities learned in course as

$$2A_1^T A_1 A_1^T A_1 x \quad (0.5 \text{ marks})$$

Next we can see that

$$\|A_2^T x\|_2^2 = x^T A_2 A_2^T x \quad (0.5 \text{ marks})$$

The gradient of the above part alone is easily derived based on identities learned in course as

$$2A_2A_2^T x \quad (0.5 \text{ marks})$$

$$\text{In summary } \nabla g(x) = 2A_1^T A_1 A_1^T A_1 x + 2A_2 A_2^T x$$

Q3 Alternative approaches would also be accepted and awarded marks

a i)

$$\det(\mathbf{A} - \lambda \mathbf{I}) = 0$$

$$\Rightarrow (1 - \lambda)(\lambda^2 - 2\lambda + (1 - 2\rho^2)) = 0 \quad (0.5 \text{ marks})$$

$$\Rightarrow \lambda = 1, 1 \pm \rho\sqrt{2} \quad (1.5 \text{ marks})$$

Now for \mathbf{A} to be positive definite all eigenvalues need to be positive as $\mathbf{A} = \mathbf{A}^T$. Therefore, we have

$$1 \pm \rho\sqrt{2} > 0$$

$$\Rightarrow 1 + \rho\sqrt{2} > 0 \text{ and } 1 - \rho\sqrt{2} > 0$$

$$\Rightarrow \frac{-1}{\sqrt{2}} < \rho < \frac{1}{\sqrt{2}} \quad (1 \text{ mark})$$

Thus, $\langle \mathbf{x}, \mathbf{y} \rangle_{\mathbf{A}} = \mathbf{x}^T \mathbf{A} \mathbf{y}$ is an innerproduct defined on \mathbb{R}^3 if $\frac{-1}{\sqrt{2}} < \rho < \frac{1}{\sqrt{2}}$.

a ii)

$$\begin{aligned} \langle \mathbf{x}, \mathbf{y} \rangle_{\mathbf{A}} &= \begin{pmatrix} 1 & 0 & 0 \end{pmatrix} \begin{pmatrix} 1 & 0 & \rho \\ 0 & 1 & \rho \\ \rho & \rho & 1 \end{pmatrix} \begin{pmatrix} 0 \\ 1 \\ 0 \end{pmatrix} \quad (0.5 \text{ mark}) \\ &= 0. \quad (0.5 \text{ mark}) \end{aligned}$$

Let $\mathbf{z} = [z_1, z_2, z_3]^T$. \mathbf{z} perpendicular to \mathbf{x} will give us

$$\begin{aligned} \langle \mathbf{x}, \mathbf{z} \rangle_{\mathbf{A}} &= 0 \\ \Rightarrow \begin{pmatrix} 1 & 0 & 0 \end{pmatrix} \begin{pmatrix} 1 & 0 & \rho \\ 0 & 1 & \rho \\ \rho & \rho & 1 \end{pmatrix} \begin{pmatrix} z_1 \\ z_2 \\ z_3 \end{pmatrix} &= 0 \\ z_1 + \rho z_3 &= 0 \quad (0.5 \text{ marks}) \end{aligned}$$

\mathbf{z} perpendicular to \mathbf{y} will give us

$$\begin{aligned} \langle \mathbf{y}, \mathbf{z} \rangle_{\mathbf{A}} &= 0 \\ \Rightarrow \begin{pmatrix} 0 & 1 & 0 \end{pmatrix} \begin{pmatrix} 1 & 0 & \rho \\ 0 & 1 & \rho \\ \rho & \rho & 1 \end{pmatrix} \begin{pmatrix} z_1 \\ z_2 \\ z_3 \end{pmatrix} &= 0 \\ z_2 + \rho z_3 &= 0 \quad (0.5 \text{ marks}) \end{aligned}$$

The augmented matrix corresponding to the system of two equations can be written as $\left(\begin{array}{ccc|c} 1 & 0 & \rho & 0 \\ 0 & 1 & \rho & 0 \end{array}\right)$. (0.5 marks)

Now putting $z_3 = t$, we get $z_1 = z_2 = -\rho t$.

Therefore $\mathbf{z} = \begin{pmatrix} -\rho t \\ -\rho t \\ t \end{pmatrix}$, $\forall t \in \mathbb{R}$. (0.5 marks)

b i) Now $\nabla_{\mathbf{x}} f = \begin{pmatrix} \mathbf{x}^T(\mathbf{Q} + \mathbf{Q}^T) \\ \mathbf{b}^T \end{pmatrix} = \begin{pmatrix} 2\mathbf{x}^T \mathbf{Q} \\ \mathbf{b}^T \end{pmatrix}$ as \mathbf{Q} is symmetric. (1 mark)

b ii)

$$f(0, 0, 0) = \begin{pmatrix} [0, 0, 0] \mathbf{Q} [0, 0, 0]^T \\ \mathbf{b}^T [0, 0, 0]^T \end{pmatrix} = \begin{pmatrix} 0 \\ 0 \end{pmatrix}. \text{ (0.5 marks)}$$

$$\nabla_{\mathbf{x}} f(0, 0, 0) = \begin{pmatrix} 2[0, 0, 0] \mathbf{Q} \\ \mathbf{b}^T \end{pmatrix} = \begin{pmatrix} \mathbf{0}^T \\ \mathbf{b}^T \end{pmatrix}. \text{ (0.5 marks)}$$

where $\mathbf{0}^T = (0, 0, 0)$.

The linear approximation of f about $(0, 0, 0)$ is given by

$$\begin{aligned} T_1 f(\mathbf{x}) &= f(0, 0, 0) + \nabla_{\mathbf{x}} f(0, 0, 0) \mathbf{x} \\ &= \begin{pmatrix} 0 \\ 0 \end{pmatrix} + \begin{pmatrix} \mathbf{0}^T \\ \mathbf{b}^T \end{pmatrix} \mathbf{x} = \begin{pmatrix} 0 \\ \mathbf{b}^T \mathbf{x} \end{pmatrix} \end{aligned}$$

(1 mark)

c Let $\mathbf{M} = \begin{pmatrix} a & b \\ c & d \end{pmatrix}$

So, the problem is to $\min(\|\mathbf{M} - \mathbf{A}\|_2)^2 = (a - 1)^2 + b^2 + c^2 + (d - 2)^2$ such that $a + d = 0$. (0.5 marks)

Therefore, the Lagrangian of the constrained optimization problem is given by

$$L(a, b, c, d, \lambda) = (a - 1)^2 + b^2 + c^2 + (d - 2)^2 + \lambda(a + d) \text{ (0.5 marks)}$$

Partially differentiating with respect to a, b, c, d, λ , we get

$$\begin{aligned} \frac{\partial L}{\partial a} &= 2a - 2 + \lambda = 0 \Rightarrow a = \frac{-\lambda + 2}{2}, \\ \frac{\partial L}{\partial b} &= 2b = 0 \Rightarrow b = 0, \\ \frac{\partial L}{\partial c} &= 2c = 0 \Rightarrow c = 0, \\ \frac{\partial L}{\partial d} &= 2d - 4 + \lambda = 0 \Rightarrow d = \frac{-\lambda + 4}{2} \\ \frac{\partial L}{\partial \lambda} &= a + d = 0 \Rightarrow \lambda = 3 \end{aligned}$$

(0.5 marks for a, d in terms of λ , 0.5 marks for $b = c = 0$, 0.5 marks for finding value of λ)

Thus, $\mathbf{M} = \begin{pmatrix} \frac{-1}{2} & 0 \\ 0 & \frac{1}{2} \end{pmatrix}$ (0.5 marks)